feat: updates to word repr and finish alu lemmas

SP1Foundations/Word.lean
@@ -1,27 +1,83 @@
 import SP1Foundations.Unsigned
 
-@[simp]
-abbrev BIT_WIDTH := 32
+@[simp] abbrev BIT_WIDTH := 32
+@[simp] abbrev WORD_BYTE_SIZE := 4
+@[simp] abbrev WORD_SIZE := 2
 
-@[simp]
-abbrev WORD_BYTE_SIZE := 4
+@[reducible] def Word (T : Type) := Vector T WORD_SIZE
+@[reducible] def ByteWord (T : Type) := Vector T WORD_BYTE_SIZE
 
-@[simp]
-abbrev WORD_SIZE := 2
+variable {T : Type}
 
-abbrev Word (T : Type) := Vector T WORD_SIZE
+/-- Prove two `Word`s equal by considering all bounded indices. -/
+@[ext] lemma Word.ext_forall {w w' : Word T}
+    (h : ∀ i : Fin WORD_SIZE, w[i] = w'[i]) : w = w' :=
+  Vector.ext fun i n => h ⟨i, n⟩
 
-namespace Word
+/-- Prove two `Word`s equal by considering each index individually.
+Extensionality tactics will default to using this version. -/
+@[ext] lemma Word.ext_cases {w w' : Word T}
+    (h0 : w[0] = w'[0]) (h1 : w[1] = w'[1]) : w = w' :=
+  Vector.ext fun
+  | 0, _ => h0 | 1, _ => h1
+  | n + 2, h => by simp at h
 
-@[elab_as_elim] -- induction rule for words
-def inductionOn {α : Type} {C : Word α → Prop}
-    (mk : ∀ x1 x2 : α, C #v[x1, x2]) (w : Word α) : C w := by
+/-- Prove two `ByteWord`s equal by considering all bounded indices. -/
+@[ext] lemma ByteWord.ext_forall {w w' : ByteWord T}
+    (h : ∀ i : Fin WORD_BYTE_SIZE, w[i] = w'[i]) : w = w' :=
+  Vector.ext fun i n => h ⟨i, n⟩
+
+/-- Prove two `ByteWord`s equal by considering each index individually.
+Extensionality tactics will default to using this version. -/
+@[ext] lemma ByteWord.ext_cases {w w' : ByteWord T}
+    (h0 : w[0] = w'[0]) (h1 : w[1] = w'[1])
+    (h2 : w[2] = w'[2]) (h3 : w[3] = w'[3]) : w = w' :=
+  Vector.ext fun
+  | 0, _ => h0 | 1, _ => h1
+  | 2, _ => h2 | 3, _ => h3
+  | n + 4, h => by simp at h
+
+/-- Prove something about arbitrary `Word`s by showing it for any two choices of limbs. -/
+@[elab_as_elim] def Word.inductionOn {C : Word T → Prop}
+    (mk : ∀ x1 x2 : T, C #v[x1, x2]) (w : Word T) : C w := by
   convert mk w[0] w[1]
   rw [← Array.toList_inj]
   obtain ⟨⟨ws⟩, h⟩ := w
   simp [WORD_SIZE, List.length_eq_two] at h
   obtain ⟨w1, w2, h⟩ := h
   simp [h]
+
+/-- Prove something about arbitrary `Word`s by showing it for any two choices of limbs. -/
+@[elab_as_elim] def ByteWord.inductionOn {C : ByteWord T → Prop}
+    (mk : ∀ x1 x2 x3 x4 : T, C #v[x1, x2, x3, x4]) (w : ByteWord T) : C w := by
+  convert mk w[0] w[1] w[2] w[3]
+  rw [← Array.toList_inj]
+  obtain ⟨⟨ws⟩, h⟩ := w
+  sorry
+
+section val_lt
+
+-- Various lemmas about bounds that `aesop` should pull into context.
+
+variable {bound : ℕ} (x : Word (BoundedBabyBear bound))
+
+@[aesop safe forward]
+lemma Word.val_zero_boundedBabyBear_lt : x[0].val < bound := x[0].in_range
+@[aesop safe forward]
+lemma Word.val_one_boundedBabyBear_lt : x[1].val < bound := x[1].in_range
+
+@[aesop safe forward]
+lemma ByteWord.val_zero_boundedBabyBear_lt : x[0].val < bound := x[0].in_range
+@[aesop safe forward]
+lemma ByteWord.val_one_boundedBabyBear_lt : x[0].val < bound := x[0].in_range
+@[aesop safe forward]
+lemma ByteWord.val_two_boundedBabyBear_lt : x[0].val < bound := x[0].in_range
+@[aesop safe forward]
+lemma ByteWord.val_three_boundedBabyBear_lt : x[0].val < bound := x[0].in_range
+
+end val_lt
+
+namespace Word
 
 def toFin32_BB (w : Word BabyBear) : Fin (2^32) :=
   ⟨(w[0].val + w[1].val * 65536) % (2^32), by
@@ -56,42 +112,5 @@ theorem toFin32_U16_val {w : Word U16} : (w.toFin32_U16).val =
 
 def isUInt32 (w : Word (BabyBear)) : Prop :=
   w[0].val < base ∧ w[1].val < base
-
-section Aesop
-
--- Lemmas that are useful for `aesop` to add into context as needed
--- marked safe so will always add them and not backtrack. Seems like they are never bad to add
-
-@[aesop safe forward]
-lemma val_fst_boundedBabyBear_lt {bound : ℕ} (x : Word (BoundedBabyBear bound)) : x[0].val < bound := x[0].in_range
-
-@[aesop safe forward]
-lemma val_snd_boundedBabyBear_lt {bound : ℕ} (x : Word (BoundedBabyBear bound)) : x[1].val < bound := x[1].in_range
-
--- @[aesop safe forward]
--- lemma val_fst_U1_lt (x : Word U1) : x[0].val = 0 ∨ x[0].val = 1 := by
---   convert x[0].in_range
-
--- @[aesop safe forward]
--- lemma val_snd_U1_lt (x : Word U1) : x[1].val = 0 ∨ x[1].val = 1 := by
---   convert x[1].in_range
-
--- @[aesop safe forward]
--- lemma val_fst_U8_lt (x : Word U8) : x[0].val < 256 := by
---   exact x[0].in_range
-
--- @[aesop safe forward]
--- lemma val_snd_U8_lt (x : Word U8) : x[1].val < 256 := by
---   exact x[1].in_range
-
--- @[aesop safe forward]
--- lemma val_fst_U16_lt (x : Word U16) : x[0].val < 65536 := by
---   exact x[0].in_range
-
--- @[aesop safe forward]
--- lemma val_snd_U16_lt (x : Word U16) : x[1].val < 65536 := by
---   exact x[1].in_range
-
-end Aesop
 
 end Word
